deps/poulet4/lib/P4cub/Syntax/AST.v
@@ -4,405 +4,288 @@ Require Import Coq.PArith.BinPosDef Coq.PArith.BinPos
 Require Export Poulet4.P4cub.Syntax.P4Field.
 Require Coq.Logic.Eqdep_dec.
 Import String.
+
 (** * P4cub AST *)
 
-Module F := Field.
+(** De Bruijn syntax. *)
 
 (** Function call parameters/arguments. *)
-Variant paramarg (A B : Type) : Type :=
-| PAIn (a : A)
-| PAOut (b : B)
-| PAInOut (b : B)
-| PADirLess (a : A).
+Variant paramarg (A B : Set) : Set :=
+| PAIn      (a : A) (** in-parameter. *)
+| PAOut     (b : B) (** out-parameter. *)
+| PAInOut   (b : B) (** inout-parameter. *)
+| PADirLess (a : A) (** direction-less parameter *).
 
 Arguments PAIn {_} {_}.
 Arguments PAOut {_} {_}.
 Arguments PAInOut {_} {_}.
 Arguments PADirLess {_} {_}.
 
-Definition paramarg_map {A B C D : Type}
+Definition paramarg_map {A B C D : Set}
            (f : A -> C) (g : B -> D)
            (pa : paramarg A B) : paramarg C D :=
   match pa with
-  | PAIn a => PAIn (f a)
-  | PAOut b => PAOut (g b)
-  | PAInOut b => PAInOut (g b)
+  | PAIn      a => PAIn      (f a)
+  | PAOut     b => PAOut     (g b)
+  | PAInOut   b => PAInOut   (g b)
   | PADirLess a => PADirLess (f a)
   end.
-(**[]*)
 
 (** A predicate on a [paramarg]. *)
-Definition pred_paramarg {A B : Type}
+Definition pred_paramarg {A B : Set}
            (PA : A -> Prop) (PB : B -> Prop) (pa : paramarg A B) : Prop :=
   match pa with
-  | PAIn a | PADirLess a => PA a
-  | PAOut b | PAInOut b => PB b
+  | PAIn  a | PADirLess a => PA a
+  | PAOut b | PAInOut   b => PB b
   end.
-(**[]*)
 
-Definition pred_paramarg_same {A : Type} (P : A -> Prop)
+Definition pred_paramarg_same {A : Set} (P : A -> Prop)
   : paramarg A A -> Prop := pred_paramarg P P.
-(**[]*)
 
 (** Relating [paramarg]s. *)
-Definition rel_paramarg {A1 A2 B1 B2 : Type}
+Definition rel_paramarg {A1 A2 B1 B2 : Set}
            (RA : A1 -> A2 -> Prop) (RB : B1 -> B2 -> Prop)
            (pa1 : paramarg A1 B1)
            (pa2 : paramarg A2 B2) : Prop :=
   match pa1, pa2 with
   | PADirLess a1, PADirLess a2 
-  | PAIn a1, PAIn a2       => RA a1 a2
-  | PAOut b1, PAOut b2
-  | PAInOut b1, PAInOut b2 => RB b1 b2
-  | _, _ => False
+  | PAIn      a1, PAIn      a2 => RA a1 a2
+  | PAOut     b1, PAOut     b2
+  | PAInOut   b1, PAInOut   b2 => RB b1 b2
+  | _           , _            => False
   end.
-(**[]*)
 
-Definition rel_paramarg_same {A B : Type} (R : A -> B -> Prop) :
+Definition rel_paramarg_same {A B : Set} (R : A -> B -> Prop) :
   paramarg A A -> paramarg B B -> Prop :=
   rel_paramarg R R.
-(**[]*)
 
 (** Function signatures/instantiations. *)
-Record arrow (K A B R : Type) : Type :=
-  { paramargs : F.fs K (paramarg A B);
-    rtrns : option R }.
-(**[]*)
+Record arrow (A B : Set) : Set :=
+  { paramargs : list (paramarg A B);
+    rtrns : option B }.
 
-Arguments paramargs {_} {_} {_} {_}.
-Arguments rtrns {_} {_} {_} {_}.
+Arguments paramargs {_} {_}.
+Arguments rtrns {_} {_}.
 
 (** * Expression Grammar *)
 Module Expr.
-  Section P4Types.
-    (** Expression types. *)
-    Inductive t : Type :=
-    | TBool                            (* bool *)
-    | TBit (width : N)                 (* unsigned integers *)
-    | TInt (width : positive)          (* signed integers *)
-    | TError                           (* the error type *)
-    | TTuple (types : list t)          (* tuple type *)
-    | TStruct (fields : F.fs string t) (* the struct and struct type *)
-    | THeader (fields : F.fs string t) (* the header type *)
-    | THeaderStack (fields : F.fs string t)
-                   (size : positive)   (* header stack type *)
-    | TVar (type_name : string)        (* type variables *).
-    (**[]*)
+  (** Expression types. *)
+  Inductive t : Set :=
+  | TBool                     (** bool *)
+  | TBit (width : N)          (** unsigned integers *)
+  | TInt (width : positive)   (** signed integers *)
+  | TError                    (** the error type *)
+  | TStruct (fields : list t)
+            (isheader : bool)    (** struct types *)
+  | TVar (type_name : nat)      (** type variables *).  
     
-    (** Function parameters. *)
-    Definition params : Type := F.fs string (paramarg t t).
+  (** Function parameters. *)
+  Definition params : Set := list (paramarg t t).
     
-    (** Function types. *)
-    Definition arrowT : Type := arrow string t t t.
+  (** Function types. *)
+  Definition arrowT : Set := arrow t t.
     
-    (** Constructor Types. *)
-    Inductive ct : Type :=
-    | CTType (type : t)                   (* expression types *)
-    | CTControl (cparams : F.fs string ct)
-                (runtime_extern_params : F.fs string string)
-                (parameters : params)     (* control types *)
-    | CTParser (cparams : F.fs string ct)
-               (runtime_extern_params : F.fs string string)
-               (parameters : params)      (* parser types *)
-    | CTPackage (cparams : F.fs string ct) (* package types *)
-    | CTExtern (extern_name : string).
-    (**[]*)
+  (** Constructor types. *)
+  Inductive ct : Set :=
+  | CTType (type : t)              (** expression types *)
+  | CTControl (cparams : list ct)
+              (runtime_extern_params : list string)
+              (parameters : params)(** control types *)
+  | CTParser (cparams : list ct)
+             (runtime_extern_params : list string)
+             (parameters : params) (** parser types *)
+  | CTPackage (cparams : list ct)  (** package types *)
+  | CTExtern (extern_name : string).  
     
-    Definition constructor_params : Type := F.fs string ct.
-  End P4Types.
+  Definition constructor_params : Set := list ct.
   
   Variant uop : Set :=
-  | Not        (* boolean negation *)
-  | BitNot     (* bitwise negation *)
-  | UMinus     (* integer negation *)
-  | IsValid    (* check header validity *)
-  | SetValid   (* set a header valid *)
-  | SetInValid (* set a header invalid *)
-  | NextIndex  (* get element at [nextIndex] from a header stack *)
-  | Size       (* get a header stack's size *).
-  (**[]*)
+    | Not        (** boolean negation *)
+    | BitNot     (** bitwise negation *)
+    | UMinus     (** integer negation *)
+    | IsValid    (** check header validity *)
+    | SetValid   (** set a header valid *)
+    | SetInValid (** set a header invalid *)
+    | NextIndex  (** get element at [nextIndex] from a header stack *)
+    | Size       (** get a header stack's size *).  
   
   (** Binary operations.
       The "Sat" suffix denotes
       saturating arithmetic:
       where there is no overflow. *)
   Variant bop : Set :=
-  | Plus     (* integer addition *)
-  | PlusSat  (* saturating addition *)
-  | Minus    (* integer subtraction *)
-  | MinusSat (* saturating subtraction *)
-  | Times    (* multiplication *)
-  | Shl      (* bitwise left-shift *)
-  | Shr      (* bitwise right-shift *)
-  | Le       (* integer less-than *)
-  | Ge       (* integer greater-than *)
-  | Lt       (* integer less-than or equals *)
-  | Gt       (* integer greater-than or equals *)
-  | Eq       (* expression equality *)
-  | NotEq    (* expression inequality *)
-  | BitAnd   (* bitwise and *)
-  | BitXor   (* bitwise exclusive-or *)
-  | BitOr    (* bitwise or *)
-  | PlusPlus (* bit-string concatenation *)
-  | And      (* boolean and *)
-  | Or       (* boolean or *).
-  (**[]*)
-  
-  (** Default matchkinds. *)
-  Variant matchkind : Set :=
-  | MKExact
-  | MKTernary
-  | MKLpm.
-  (**[]*)
-  
-  Section Expressions.
-    Variable (tags_t : Type).
+  | Plus     (** integer addition *)
+  | PlusSat  (** saturating addition *)
+  | Minus    (** integer subtraction *)
+  | MinusSat (** saturating subtraction *)
+  | Times    (** multiplication *)
+  | Shl      (** bitwise left-shift *)
+  | Shr      (** bitwise right-shift *)
+  | Le       (** integer less-than *)
+  | Ge       (** integer greater-than *)
+  | Lt       (** integer less-than or equals *)
+  | Gt       (** integer greater-than or equals *)
+  | Eq       (** expression equality *)
+  | NotEq    (** expression inequality *)
+  | BitAnd   (** bitwise and *)
+  | BitXor   (** bitwise exclusive-or *)
+  | BitOr    (** bitwise or *)
+  | PlusPlus (** bit-string concatenation *)
+  | And      (** boolean and *)
+  | Or       (** boolean or *).
 
-    (* AST parameterized by variable type.
-       variable type needs decidable equality (or an order).
-       order is faster then membership checking. *)
+  (** Expressions annotated with types,
+      unless the type is obvious. *)
+  
+  Inductive e : Set :=
+  | EBool (b : bool)                      (** booleans *)
+  | EBit (width : N) (val : Z)         (** unsigned integers *)
+  | EInt (width : positive) (val : Z)  (** signed integers *)
+  | EVar (type : t) (x : nat)            (** variables *)
+  | ESlice (arg : e)
+           (hi lo : positive)          (** bit-slicing *)
+  | ECast (type : t) (arg : e)         (** explicit casts *)
+  | EUop (result_type : t) (op : uop)
+         (arg : e)                     (** unary operations *)
+  | EBop (result_type : t) (op : bop)
+         (lhs rhs : e)                 (** binary operations *)
+  | EStruct (fields : list e) (valid : option e) (** struct literals *)
+  | EExprMember (result_type : t) (mem : nat)
+                (arg : e)              (** member-expressions *)
+  | EError (err : option string)       (** error literals *).    
+  
+  (** Function call arguments. *)
+  Definition args : Set := list (paramarg e e).
     
-    (** Expressions annotated with types,
-        unless the type is obvious. *)
-    Inductive e : Type :=
-    | EBool (b : bool) (i : tags_t)                     (* booleans *)
-    | EBit (width : N) (val : Z) (i : tags_t)        (* unsigned integers *)
-    | EInt (width : positive) (val : Z) (i : tags_t) (* signed integers *)
-    | EVar (type : t) (x : string) (i : tags_t)      (* variables *)
-    | ESlice (arg : e)
-             (hi lo : positive) (i : tags_t)         (* bit-slicing *)
-    | ECast (type : t) (arg : e) (i : tags_t)        (* explicit casts *)
-    | EUop (result_type : t) (op : uop)
-           (arg : e) (i : tags_t)                    (* unary operations *)
-    | EBop (result_type : t) (op : bop)
-           (lhs rhs : e) (i : tags_t)                (* binary operations *)
-    | ETuple (es : list e) (i : tags_t)              (* tuples *)
-    | EStruct (fields : F.fs string e) (i : tags_t)  (* struct literals *)
-    | EHeader (fields : F.fs string e)
-              (valid : e) (i : tags_t)               (* header literals *)
-    | EExprMember (result_type : t) (mem : string)
-                  (arg : e) (i : tags_t)             (* member-expressions *)
-    | EError (err : option string) (i : tags_t)      (* error literals *)
-    | EHeaderStack (fields : F.fs string t)
-                   (headers : list e)                (* header stack literals *)
-                   (next_index : Z) (i : tags_t)     (*unique to p4cub *)
-    | EHeaderStackAccess (result_hdr_type : F.fs string t)
-                         (stk : e)
-                         (index : Z) (i : tags_t)    (* header stack indexing *).
-    (**[]*)
+  (** Function call. *)
+  Definition arrowE : Set := arrow e e.
     
-    (** Function call arguments. *)
-    Definition args : Type :=
-      F.fs string (paramarg e e).
-    (**[]*)
+  (** Constructor arguments. *)
+  Variant constructor_arg : Set :=
+    | CAExpr (expr : e)   (** plain expression *)
+    | CAName (x : nat)      (** name of parser, control, package, or extern *).
     
-    (** Function call. *)
-    Definition arrowE : Type :=
-      arrow string e e e.
-    (**[]*)
-    
-    (** Constructor arguments. *)
-    Variant constructor_arg : Type :=
-    | CAExpr (expr : e)   (* plain expression *)
-    | CAName (x : string) (* name of parser, control, package, or extern *).
-    (**[]*)
-    
-    Definition constructor_args : Type := F.fs string constructor_arg.
-  End Expressions.
-
-  Arguments EBool {tags_t}.
-  Arguments EBit {_}.
-  Arguments EInt {_}.
-  Arguments EVar {tags_t}.
-  Arguments ESlice {_}.
-  Arguments ECast {_}.
-  Arguments EUop {tags_t}.
-  Arguments EBop {tags_t}.
-  Arguments ETuple {_}.
-  Arguments EStruct {tags_t}.
-  Arguments EHeader {_}.
-  Arguments EExprMember {tags_t}.
-  Arguments EError {tags_t}.
-  Arguments EHeaderStack {_}.
-  Arguments EHeaderStackAccess {_}.
-  Arguments CAExpr {_}.
-  Arguments CAName {_}.
+  Definition constructor_args : Set := list constructor_arg.
 End Expr.
 
 (** Statement Grammar *)
 Module Stmt.
-  Section Statements.
-    Variable (tags_t : Type).
-
-    (** Header Stack Operations. *)
-    Variant hsop : Set := HSPush | HSPop.
-
-    Inductive s : Type :=
-    | SSkip (i : tags_t)                         (* skip/no-op *)
-    | SVardecl (x : string) (expr : Expr.t + Expr.e tags_t)
-               (i : tags_t)                      (* variable declaration. *)
-    | SAssign (lhs rhs : Expr.e tags_t) (i : tags_t)     (* assignment *)
-    | SConditional (guard : Expr.e tags_t)
-                   (tru_blk fls_blk : s) (i : tags_t) (* conditionals *)
-    | SSeq (s1 s2 : s) (i : tags_t)                   (* sequences *)
-    | SBlock (blk : s)                                (* blocks *)
-    | SExternMethodCall (extern_name method_name : string)
-                        (typ_args : list Expr.t)
-                        (args : Expr.arrowE tags_t)
-                        (i : tags_t)             (* extern method calls *)
-    | SFunCall (f : string)
-               (typ_args : list Expr.t)
-               (args : Expr.arrowE tags_t) (i : tags_t) (* function call *)
-    | SActCall (action_name : string)
-               (args : Expr.args tags_t) (i : tags_t) (* action call *)
-    | SReturn (e : option (Expr.e tags_t))
-              (i : tags_t)                          (* return statement *)
-    | SExit (i : tags_t)                            (* exit statement *)
-    | SInvoke (table_name : string) (i : tags_t)    (* table invocation *)
-    | SApply (instance_name : string)
-             (ext_args : F.fs string string)
-             (args : Expr.args tags_t)
-             (i : tags_t) (* apply statements *)
-    | SHeaderStackOp (hdr_stk_name : string) (hdr_typ : Expr.t) (o : hsop)
-                     (n : positive) (i : tags_t)  (* push/pop statements *)
-    | SSetValidity (hdr : Expr.e tags_t) (validity : bool)
-                   (i : tags_t)               (* set valid or set invalid *).
-  (**[]*)
-  End Statements.
-
-  Arguments SSkip {tags_t}.
-  Arguments SVardecl {_}.
-  Arguments SAssign {tags_t}.
-  Arguments SConditional {tags_t}.
-  Arguments SSeq {tags_t}.
-  Arguments SBlock {_}.
-  Arguments SFunCall {_}.
-  Arguments SActCall {_}.
-  Arguments SExternMethodCall {_}.
-  Arguments SReturn {_}.
-  Arguments SExit {_}.
-  Arguments SApply {_}.
-  Arguments SInvoke {_}.
-  Arguments SHeaderStackOp {_}.
-  Arguments SSetValidity {_}.
+  Inductive s : Set :=
+  | SSkip (** skip/no-op *)
+  | SVardecl
+      (x : nat) (expr : Expr.t + Expr.e) (** variable declaration. *)
+  | SAssign (lhs rhs : Expr.e) (** assignment *)
+  | SConditional
+      (guard : Expr.e)
+      (tru_blk fls_blk : s) (** conditionals *)
+  | SSeq (s1 s2 : s) (** sequences *)
+  | SBlock (blk : s) (** blocks *)
+  | SExternMethodCall
+      (extern_name method_name : string)
+      (typ_args : list Expr.t)
+      (args : Expr.arrowE ) (** extern method calls *)
+  | SFunCall
+      (f : string)
+      (typ_args : list Expr.t)
+      (args : Expr.arrowE)  (** function call *)
+  | SActCall
+      (action_name : string)
+      (args : Expr.args) (** action call *)
+  | SReturn (e : option Expr.e) (** return statement *)
+  | SExit (** exit statement *)
+  | SInvoke (table_name : string) (** table invocation *)
+  | SApply (instance_name : string)
+           (ext_args : list string)
+           (args : Expr.args) (** apply statements *).
 End Stmt.
 
 (** Parsers *)
 Module Parser.
   (** Labels for parser-states. *)
   Variant state : Set :=
-  | STStart              (* start state *)
-  | STAccept             (* accept state *)
-  | STReject             (* reject state *)
-  | STName (st : string) (* user-defined state *).
-  (**[]*)
+    | STStart         (** start state *)
+    | STAccept        (** accept state *)
+    | STReject        (** reject state *)
+    | STName (st : nat) (** user-defined state *).
 
   (** Select expression pattern.
       Corresponds to keySet expressions in p4. *)
-  Inductive pat : Type :=
-  | PATWild                             (* wild-card/anything pattern *)
-  | PATMask (p1 p2 : pat)               (* mask pattern *)
-  | PATRange (p1 p2 : pat)              (* range pattern *)
-  | PATBit (width : N) (val : Z)        (* unsigned-int pattern *)
-  | PATInt (width : positive) (val : Z) (* signed-int pattern *)
-  | PATTuple (ps : list pat).           (* tuple pattern *)
-  (**[]*)
+  Inductive pat : Set :=
+  | PATWild                             (** wild-card/anything pattern *)
+  | PATMask (p1 p2 : pat)               (** mask pattern *)
+  | PATRange (p1 p2 : pat)              (** range pattern *)
+  | PATBit (width : N) (val : Z)        (** unsigned-int pattern *)
+  | PATInt (width : positive) (val : Z) (** signed-int pattern *)
+  | PATTuple (ps : list pat)            (** tuple pattern *).
 
-  Section Parsers.
-    Variable (tags_t : Type).
-
-    (** Parser expressions, which evaluate to state names *)
-    Inductive e : Type :=
-    | PGoto (st : state) (i : tags_t) (* goto state [st] *)
-    | PSelect (discriminee : Expr.e tags_t)
-              (default : e) (cases : F.fs pat e)
-              (i : tags_t)           (* select expressions,
-                                        where "default" is
-                                        the catch-all case *).
-    (**[]*)
-
-    (** Parser State Blocks. *)
-    Record state_block : Type :=
-      { stmt : Stmt.s tags_t; trans : e }.
-    (**[]*)
-  End Parsers.
-
-  Arguments stmt {_}.
-  Arguments trans {_}.
-  Arguments PGoto {_}.
-  Arguments PSelect {_}.
+  (** Parser expressions, which evaluate to state names *)
+  Inductive e : Set :=
+  | PGoto (st : state)  (** goto state [st] *)
+  | PSelect (discriminee : Expr.e)
+            (default : e) (cases : Field.fs pat e)
+                       (** select expressions,
+                                       where "default" is
+                                       the catch-all case *).
+  
+  (** Parser State Blocks. *)
+  Record state_block : Set :=
+    { stmt : Stmt.s ; trans : e }.
 End Parser.
 
 (** Controls *)
 Module Control.
-  Section ControlDecls.
-    Variable (tags_t : Type).
+  (** Table. *)
+  Record table : Set :=
+    { table_key : list (Expr.e * string); 
+      table_actions : list string }.
     
-    (** Table. *)
-    Record table : Type :=
-      { table_key : list (Expr.e tags_t * Expr.matchkind); 
-        table_actions : list string }.
-    (**[]*)
-    
-    (** Declarations that may occur within Controls. *)
-    Inductive d : Type :=
-    | CDAction (action_name : string)
-               (signature : Expr.params) (body : Stmt.s tags_t)
-               (i : tags_t)               (* action declaration *)
-    | CDTable (table_name : string)
-              (body : table) (i : tags_t) (* table declaration *)
-    | CDSeq (d1 d2 : d) (i : tags_t)      (* sequence of declarations *).
-    (**[]*)
-  End ControlDecls.
-
-  Arguments table_key {_}.
-  Arguments table_actions {_}.
-  Arguments CDAction {_}.
-  Arguments CDTable {_}.
-  Arguments CDSeq {_}.
+  (** Declarations that may occur within Controls. *)
+  Inductive d : Set :=
+  | CDAction (action_name : string)
+             (signature : Expr.params) (body : Stmt.s )
+  (** action declaration *)
+  | CDTable (table_name : string)
+            (body : table)  (** table declaration *)
+  | CDSeq (d1 d2 : d)       (** sequence of declarations *).
 End Control.
 
 (** Top-Level Declarations *)
 Module TopDecl.
-  Section TopDeclarations.
-    Variable (tags_t : Type).
-
-    (** Top-level declarations. *)
-    Inductive d : Type :=
-    | TPInstantiate (constructor_name instance_name : string)
-                    (type_args : list Expr.t)
-                    (cargs : Expr.constructor_args tags_t)
-                    (i : tags_t) (* instantiations *)
-    | TPExtern (extern_name : string)
-               (type_params : list string)
-               (cparams : Expr.constructor_params)
-               (methods : F.fs string (list string * Expr.arrowT))
-               (i : tags_t) (* extern declarations *)
-    | TPControl (control_name : string)
-                (cparams : Expr.constructor_params) (* constructor params *)
-                (eparams : F.fs string string)   (* runtime extern params *)
-                (params : Expr.params)              (* apply block params *)
-                (body : Control.d tags_t) (apply_blk : Stmt.s tags_t)
-                (i : tags_t) (* control declarations *)
-    | TPParser (parser_name : string)
-               (cparams : Expr.constructor_params) (* constructor params *)
-               (eparams : F.fs string string)   (* runtime extern params *)
-               (params : Expr.params)              (* invocation params *)
-               (start : Parser.state_block tags_t)   (* start state *)
-               (states : F.fs string (Parser.state_block tags_t)) (* parser states *)
-               (i : tags_t)  (* parser declaration *)
-    | TPFunction (function_name : string)
-                 (type_params : list string)
-                 (signature : Expr.arrowT) (body : Stmt.s tags_t)
-                 (i : tags_t)(* function/method declaration *)
-    | TPSeq (d1 d2 : d) (i : tags_t).
-    (**[]*)
-  End TopDeclarations.
-
-  Arguments TPInstantiate {_}.
-  Arguments TPExtern {_}.
-  Arguments TPControl {_}.
-  Arguments TPParser {_}.
-  Arguments TPFunction {_}.
-  Arguments TPSeq {_}.
+  (** Top-level declarations. *)
+  Inductive d : Set :=
+  | TPInstantiate
+      (constructor_name instance_name : string)
+      (type_args : list Expr.t)
+      (cargs : Expr.constructor_args )
+  (** instantiations *)
+  | TPExtern
+      (extern_name : string)
+      (type_params : nat)
+      (cparams : Expr.constructor_params)
+      (methods : Field.fs
+                   string (** method name *)
+                   (list string (** extern arguments *)
+                    * Expr.arrowT  (** parameters *) ))
+  (** extern declarations *)
+  | TPControl
+      (control_name : string)
+      (cparams : Expr.constructor_params) (** constructor params *)
+      (eparams : list string)      (** runtime extern params *)
+      (params : Expr.params)       (** apply block params *)
+      (body : Control.d ) (apply_blk : Stmt.s )
+  (** control declarations *)
+  | TPParser
+      (parser_name : string)
+      (cparams : Expr.constructor_params) (** constructor params *)
+      (eparams : list string)      (** runtime extern params *)
+      (params : Expr.params)              (** invocation params *)
+      (start : Parser.state_block ) (** start state *)
+      (states : list (Parser.state_block )) (** parser states *)
+  (** parser declaration *)
+  | TPFunction
+        (function_name : string)
+        (type_params : nat)
+        (signature : Expr.arrowT) (body : Stmt.s )
+  (** function/method declaration *)
+  | TPSeq (d1 d2 : d) .
 End TopDecl.
