deps/poulet4/lib/P4cub/Syntax/CubNotations.v
@@ -2,298 +2,144 @@ Set Warnings "-custom-entry-overridden".
 Require Import Poulet4.P4cub.Syntax.AST.
 Import String.
 
-(** Notation entries. *)
-Declare Custom Entry p4type.
-Declare Custom Entry p4constructortype.
-Declare Custom Entry p4uop.
-Declare Custom Entry p4bop.
-Declare Custom Entry p4matchkind.
-Declare Custom Entry p4expr.
-Declare Custom Entry p4hsop.
-Declare Custom Entry p4stmt.
-Declare Custom Entry p4prsrstate.
-Declare Custom Entry p4selectpattern.
-Declare Custom Entry p4prsrexpr.
-Declare Custom Entry p4prsrstateblock.
-Declare Custom Entry p4ctrldecl.
-Declare Custom Entry p4topdecl.
+Declare Scope cub_scope.
+Delimit Scope cub_scope with cub.
 
 Module TypeNotations.
   Import Expr.
-  
-  Notation "'{{' ty '}}'" := ty (ty custom p4type at level 99).
-  Notation "( x )" := x (in custom p4type, x at level 99).
-  Coercion TVar : string >-> t.
-  Notation "x" := x (in custom p4type at level 0, x constr at level 0).
-  Notation "'Bool'" := TBool (in custom p4type at level 0).
+  Coercion TVar : nat >-> t.
   Notation "'bit' < w >"
     := (TBit w)
-         (in custom p4type at level 2, no associativity).
+         (at level 2, no associativity) : cub_scope.
   Notation "'int' < w >"
     := (TInt w)
-         (in custom p4type at level 2, no associativity).
-  Notation "'error'" := TError
-                          (in custom p4type at level 0,
-                              no associativity).
-  Notation "'tuple' ts"
-    := (TTuple ts) (in custom p4type at level 0, no associativity).
-  Notation "'struct' { fields }"
-    := (TStruct fields)
-         (in custom p4type at level 6, no associativity).
-  Notation "'hdr' { fields }"
-    := (THeader fields)
-         (in custom p4type at level 6, no associativity).
-  Notation "'stack' fields [ n ]"
-    := (THeaderStack fields n) (in custom p4type at level 7).
-  
-  Notation "'{{{' ty '}}}'" := ty (ty custom p4constructortype at level 99).
-  Notation "( x )" := x (in custom p4constructortype, x at level 99).
-  Notation "x"
-    := x (in custom p4constructortype at level 0, x constr at level 0).
-  Notation "'VType' τ"
-    := (CTType τ)
-         (in custom p4constructortype at level 0,
-             τ custom p4type).
-  Notation "'ControlType' cps res ps"
-    := (CTControl cps res ps)
-         (in custom p4constructortype at level 0).
-  Notation "'ParserType' cps res ps"
-    := (CTParser cps res ps)
-         (in custom p4constructortype at level 0).
-  Notation "'PackageType' cps"
-    := (CTPackage cps)
-         (in custom p4constructortype at level 0).
-(*Notation "'Extern' cps { mthds }"
-  := (CTExtern cps mthds)
-  (in custom p4constructortype at level 0).*)
+         (at level 2, no associativity) : cub_scope.
+  Coercion CTType : t >-> ct.
 End TypeNotations.
-
-Module UopNotations.
-  Import Expr.
-  
-  Notation "'_{' u '}_'" := u (u custom p4uop at level 99).
-  Notation "( x )" := x (in custom p4uop, x at level 99).
-  Notation "x" := x (in custom p4uop at level 0, x constr at level 0).
-  Notation "!" := Not (in custom p4uop at level 0).
-  Notation "~" := BitNot (in custom p4uop at level 0).
-  Notation "-" := UMinus (in custom p4uop at level 0).
-  Notation "'isValid'" := IsValid (in custom p4uop at level 0).
-  Notation "'setValid'" := SetValid (in custom p4uop at level 0).
-  Notation "'setInValid'" := SetInValid (in custom p4uop at level 0).
-  Notation "'Next'" := NextIndex (in custom p4uop at level 0).
-  Notation "'Size'" := Size (in custom p4uop at level 0).
-End UopNotations.
-
-Module BopNotations.
-  Import Expr.
-  
-  Notation "'+{' x '}+'" := x (x custom p4bop at level 99).
-  Notation "( x )" := x (in custom p4bop, x at level 99).
-  Notation "x" := x (in custom p4bop at level 0, x constr at level 0).
-  Notation "+" := Plus (in custom p4bop at level 0).
-  Notation "-" := Minus (in custom p4bop at level 0).
-  Notation "'|+|'" := PlusSat (in custom p4bop at level 0).
-  Notation "'|-|'" := MinusSat (in custom p4bop at level 0).
-  Notation "×" := Times (in custom p4bop at level 0).
-  Notation "'<<'" := Shl (in custom p4bop at level 0).
-  Notation "'>>'" := Shr (in custom p4bop at level 0).
-  Notation "'<='" := Le (in custom p4bop at level 0).
-  Notation "'>='" := Ge (in custom p4bop at level 0).
-  Notation "<" := Lt (in custom p4bop at level 0).
-  Notation ">" := Gt (in custom p4bop at level 0).
-  Notation "'=='" := Eq (in custom p4bop at level 0).
-  Notation "'!='" := NotEq (in custom p4bop at level 0).
-  Notation "&" := BitAnd (in custom p4bop at level 0).
-  Notation "^" := BitXor (in custom p4bop at level 0).
-  Notation "|" := BitOr (in custom p4bop at level 0).
-  Notation "'&&'" := And (in custom p4bop at level 0).
-  Notation "'||'" := Or (in custom p4bop at level 0).
-  Notation "'++'" := PlusPlus (in custom p4bop at level 0).
-End BopNotations.
-
-Module MatchkindNotations.
-  Import Expr.
-  
-  Notation "'M{' x '}M'" := x (x custom p4matchkind at level 99).
-  Notation "( x )" := x (in custom p4matchkind, x at level 99).
-  Notation "x" := x (in custom p4matchkind at level 0, x constr at level 0).
-  Notation "'exact'" := MKExact (in custom p4matchkind at level 0).
-  Notation "'ternary'" := MKTernary (in custom p4matchkind at level 0).
-  Notation "'lpm'" := MKLpm (in custom p4matchkind at level 0).
-End MatchkindNotations.
 
 Module ExprNotations.
   Import Expr.
-  
-  Notation "'<{' exp '}>'" := exp (exp custom p4expr at level 99).
-  Notation "( x )" := x (in custom p4expr, x at level 99).
-  Notation "x" := x (in custom p4expr at level 0, x constr at level 0).
-  Notation "'TRUE' @ i" := (EBool true i) (in custom p4expr at level 0).
-  Notation "'FALSE' @ i" := (EBool false i) (in custom p4expr at level 0).
-  Notation "'BOOL' b @ i" := (EBool b i) (in custom p4expr at level 0).
-  Notation "w 'W' n @ i" := (EBit w n i) (in custom p4expr at level 0).
-  Notation "w 'S' n @ i" := (EInt w n i) (in custom p4expr at level 0).
-  Notation "'Var' x : ty @ i"
-    := (EVar ty x i) (in custom p4expr at level 0, no associativity).
-  Notation "'Slice' n [ hi : lo ] @ i"
-    := (ESlice n hi lo i)
-         (in custom p4expr at level 10,
-             n custom p4expr, right associativity).
-  Notation "'Cast' e : τ @ i"
-    := (ECast τ e i)
-         (in custom p4expr at level 10, τ custom p4type,
-             e custom p4expr, right associativity).
-  Notation "'UOP' op x : rt  @ i"
-    := (EUop rt op x i)
-         (in custom p4expr at level 2,
-             x custom p4expr, rt custom p4type,
-             op custom p4uop, no associativity).
-  Notation "'BOP' x op y ':' rt @ i"
-    := (EBop rt op x y i)
-         (in custom p4expr at level 10,
-             rt custom p4type,
-             x custom p4expr, y custom p4expr,
-             op custom p4bop, left associativity).
-  Notation "'tup' es @ i"
-    := (ETuple es i)
-         (in custom p4expr at level 0).
-  Notation "'struct' { fields } @ i "
-    := (EStruct fields i)
-         (in custom p4expr at level 6, no associativity).
-  Notation "'hdr' { fields } 'valid' ':=' b @ i "
-    := (EHeader fields b i)
-         (in custom p4expr at level 6,
-             b custom p4expr, no associativity).
-  Notation "'Mem' x 'dot' y ':' rt @ i"
-    := (EExprMember rt y x i)
-         (in custom p4expr at level 10, x custom p4expr,
-             rt custom p4type, left associativity).
-  Notation "'Error' x @ i"
-    := (EError x i) (in custom p4expr at level 0, no associativity).
-  Notation "'Stack' hdrs : ts 'nextIndex' ':=' ni @ i"
-    := (EHeaderStack ts hdrs ni i) (in custom p4expr at level 0).
-  Notation "'Access' e1 [ e2 ] : ts @ i"
-    := (EHeaderStackAccess ts e1 e2 i)
-         (in custom p4expr at level 10,
-             e1 custom p4expr, left associativity).
+
+  Notation "!" := Not (at level 0) : cub_scope.
+  Notation "~" := BitNot (at level 0) : cub_scope.
+  Notation "-" := UMinus (at level 0) : cub_scope.
+
+  Notation "+" := Plus (at level 0) : cub_scope.
+  Notation "-" := Minus (at level 0) : cub_scope.
+  Notation "'|+|'" := PlusSat (at level 0) : cub_scope.
+  Notation "'|-|'" := MinusSat (at level 0) : cub_scope.
+  Notation "×" := Times (at level 0) : cub_scope.
+  Notation "'<<'" := Shl (at level 0) : cub_scope.
+  Notation "'>>'" := Shr (at level 0) : cub_scope.
+  Notation "'<='" := Le (at level 0) : cub_scope.
+  Notation "'>='" := Ge (at level 0) : cub_scope.
+  Notation "<" := Lt (at level 0): cub_scope.
+  Notation ">" := Gt (at level 0): cub_scope.
+  Notation "'=='" := Eq (at level 0): cub_scope.
+  Notation "'!='" := NotEq (at level 0): cub_scope.
+  Notation "&" := BitAnd (at level 0): cub_scope.
+  Notation "^" := BitXor (at level 0): cub_scope.
+  Notation "|" := BitOr (at level 0): cub_scope.
+  Notation "'&&'" := And (at level 0): cub_scope.
+  Notation "'||'" := Or (at level 0): cub_scope.
+  Notation "'++'" := PlusPlus (at level 0): cub_scope.
+  (*Notation "w 'W' n '@' i" := (EBit w n i) (at level 0): cub_scope.
+  Notation "w 'S' n '@' i" := (EInt w n i) (at level 0): cub_scope.*)
 End ExprNotations.
 
 Module StmtNotations.
   Import Stmt.
-  
-  Notation "'<<{' sop '}>>'" := sop (sop custom p4hsop at level 99).
-  Notation "( x )" := x (in custom p4hsop, x at level 99).
-  Notation "x"
-    := x (in custom p4hsop at level 0, x constr at level 0).
-  Notation "'PUSH'" := HSPush (in custom p4hsop at level 0).
-  Notation "'POP'" := HSPop (in custom p4hsop at level 0).
-  Notation "'-{' stmt '}-'" := stmt (stmt custom p4stmt at level 99).
-  Notation "( x )" := x (in custom p4stmt, x at level 99).
-  Notation "x"
-    := x (in custom p4stmt at level 0, x constr at level 0).
-  Notation "'skip' @ i" := (SSkip i) (in custom p4stmt at level 0).
-  Notation "s1 ; s2 @ i"
+  Notation "s1 ';' s2 @ i"
     := (SSeq s1 s2 i)
-         (in custom p4stmt at level 99, s1 custom p4stmt,
-             s2 custom p4stmt, right associativity).
-  Notation "'b{' s '}b'"
-    := (SBlock s)
-         (in custom p4stmt at level 99,
-             s custom p4stmt, no associativity).
+         (at level 99, right associativity): cub_scope.
   Notation "'declare' x ':' t @ i"
     := (SVardecl x (inl t) i)
-         (in custom p4stmt at level 0,
-             t custom p4type, no associativity).
+         (at level 0, no associativity): cub_scope.
   Notation "'init' x ':=' e @ i"
     := (SVardecl x (inr e) i)
-         (in custom p4stmt at level 0,
-             e custom p4expr, no associativity).
+         (at level 0, no associativity): cub_scope.
   Notation "'var' x 'with' et @ i"
     := (SVardecl x et i)
-         (in custom p4stmt at level 0, no associativity).
+         (at level 0, no associativity): cub_scope.
   Notation "'asgn' e1 ':=' e2 @ i"
     := (SAssign e1 e2 i)
-         (in custom p4stmt at level 40,
-             e1 custom p4expr, e2 custom p4expr,
-             no associativity).
+         (at level 40, no associativity): cub_scope.
   Notation "'if' e 'then' s1 'else' s2 @ i"
     := (SConditional e s1 s2 i)
-         (in custom p4stmt at level 80,
-             s1 custom p4stmt, s2 custom p4stmt,
-             e custom p4expr, no associativity).
+         (at level 80, no associativity): cub_scope.
   Notation "'call' f < targs > ( args ) @ i"
     := (SFunCall f targs {| paramargs := args; rtrns := None |} i)
-         (in custom p4stmt at level 0, no associativity).
+         (at level 0, no associativity): cub_scope.
   Notation "'let' e ':=' 'call' f < targs > ( args ) @ i"
     := (SFunCall f targs {| paramargs := args; rtrns := Some e |} i)
-         (in custom p4stmt at level 0,
+         ( p4stmt at level 0,
              e custom p4expr, no associativity).
   Notation "'funcall' f < targs > ( args ) 'into' o @ i"
     := (SFunCall f targs {| paramargs := args; rtrns := o |} i)
-         (in custom p4stmt at level 0, no associativity).
+         ( p4stmt at level 0, no associativity).
   Notation "'calling' a 'with' args @ i"
-    := (SActCall a args i) (in custom p4stmt at level 0).
+    := (SActCall a args i) ( p4stmt at level 0).
   Notation "'extern' e 'calls' f < targs > ( args ) 'gives' x @ i"
     := (SExternMethodCall e f targs {| paramargs:=args; rtrns:=x |} i)
-         (in custom p4stmt at level 0, no associativity).
+         ( p4stmt at level 0, no associativity).
   Notation "'return' e @ i"
-    := (SReturn e i) (in custom p4stmt at level 30, no associativity).
+    := (SReturn e i) ( p4stmt at level 30, no associativity).
   Notation "'exit' @ i"
-    := (SExit i) (in custom p4stmt at level 0, no associativity).
+    := (SExit i) ( p4stmt at level 0, no associativity).
   Notation "'apply' x 'with' extargs '&' args @ i"
-    := (SApply x extargs args i) (in custom p4stmt at level 0, no associativity).
+    := (SApply x extargs args i) ( p4stmt at level 0, no associativity).
   Notation "'invoke' tbl @ i"
-    := (SInvoke tbl i) (in custom p4stmt at level 0).
+    := (SInvoke tbl i) ( p4stmt at level 0).
 End StmtNotations.
 
 Module ParserNotations.
   Import Parser.
   
   Notation "'={' st '}='" := st (st custom p4prsrstate at level 99).
-  Notation "( x )" := x (in custom p4prsrstate, x at level 99).
+  Notation "( x )" := x ( p4prsrstate, x at level 99).
   Notation "x"
-    := x (in custom p4prsrstate at level 0, x constr at level 0).
-  Notation "'start'" := STStart (in custom p4prsrstate at level 0).
-  Notation "'accept'" := STAccept (in custom p4prsrstate at level 0).
-  Notation "'reject'" := STReject (in custom p4prsrstate at level 0).
-  Notation "'δ' x" := (STName x) (in custom p4prsrstate at level 0).
+    := x ( p4prsrstate at level 0, x constr at level 0).
+  Notation "'start'" := STStart ( p4prsrstate at level 0).
+  Notation "'accept'" := STAccept ( p4prsrstate at level 0).
+  Notation "'reject'" := STReject ( p4prsrstate at level 0).
+  Notation "'δ' x" := (STName x) ( p4prsrstate at level 0).
   Notation "'[{' p '}]'" := p (p custom p4selectpattern at level 99).
-  Notation "( x )" := x (in custom p4selectpattern, x at level 99).
+  Notation "( x )" := x ( p4selectpattern, x at level 99).
   Notation "x"
-    := x (in custom p4selectpattern at level 0, x constr at level 0).
-  Notation "'??'" := PATWild (in custom p4selectpattern at level 0).
-  Notation "w 'PW' n" := (PATBit w n) (in custom p4selectpattern at level 0).
-  Notation "w 'PS' z" := (PATInt w z) (in custom p4selectpattern at level 0).
-  Notation "'PTUP' ps" := (PATTuple ps) (in custom p4selectpattern at level 0).
+    := x ( p4selectpattern at level 0, x constr at level 0).
+  Notation "'??'" := PATWild ( p4selectpattern at level 0).
+  Notation "w 'PW' n" := (PATBit w n) ( p4selectpattern at level 0).
+  Notation "w 'PS' z" := (PATInt w z) ( p4selectpattern at level 0).
+  Notation "'PTUP' ps" := (PATTuple ps) ( p4selectpattern at level 0).
   Notation "p1 '&&&' p2"
     := (PATMask p1 p2)
-         (in custom p4selectpattern at level 10,
+         ( p4selectpattern at level 10,
              p1 custom p4selectpattern, p2 custom p4selectpattern,
              right associativity).
   Notation "p1 '..' p2"
     := (PATRange p1 p2)
-         (in custom p4selectpattern at level 12,
+         ( p4selectpattern at level 12,
              p1 custom p4selectpattern, p2 custom p4selectpattern,
              right associativity).
   Notation "'p{' exp '}p'" := exp (exp custom p4prsrexpr at level 99).
-  Notation "( x )" := x (in custom p4prsrexpr, x at level 99).
+  Notation "( x )" := x ( p4prsrexpr, x at level 99).
   Notation "x"
-    := x (in custom p4prsrexpr at level 0, x constr at level 0).
+    := x ( p4prsrexpr at level 0, x constr at level 0).
   Notation "'goto' st @ i"
     := (PGoto st i)
-         (in custom p4prsrexpr at level 0,
+         ( p4prsrexpr at level 0,
              st custom p4prsrstate).
   Notation "'select' exp { cases } 'default' ':=' def @ i"
     := (PSelect exp def cases i)
-         (in custom p4prsrexpr at level 10,
+         ( p4prsrexpr at level 10,
              exp custom p4expr).
   Notation "'&{' st '}&'" := st (st custom p4prsrstateblock at level 99).
-  Notation "( x )" := x (in custom p4prsrstateblock, x at level 99).
+  Notation "( x )" := x ( p4prsrstateblock, x at level 99).
   Notation "x"
-    := x (in custom p4prsrstateblock at level 0, x constr at level 0).
+    := x ( p4prsrstateblock at level 0, x constr at level 0).
   Notation "'state' { s } 'transition' pe"
     := {| stmt:=s; trans:=pe |}
-         (in custom p4prsrstateblock at level 0,
+         ( p4prsrstateblock at level 0,
              s custom p4stmt, pe custom p4prsrexpr).
 End ParserNotations.
 
@@ -301,53 +147,53 @@ Module ControlNotations.
   Import Control.
   
   Notation "'c{' decl '}c'" := decl (decl custom p4ctrldecl at level 99).
-  Notation "( x )" := x (in custom p4ctrldecl, x at level 99).
+  Notation "( x )" := x ( p4ctrldecl, x at level 99).
   Notation "x"
-    := x (in custom p4ctrldecl at level 0, x constr at level 0).
+    := x ( p4ctrldecl at level 0, x constr at level 0).
   Notation "d1 ';c;' d2 @ i"
     := (CDSeq d1 d2 i)
-         (in custom p4ctrldecl at level 10,
+         ( p4ctrldecl at level 10,
              d1 custom p4ctrldecl, d2 custom p4ctrldecl,
              right associativity).
   Notation "'action' a ( params ) { body } @ i"
     := (CDAction a params body i)
-         (in custom p4ctrldecl at level 0, body custom p4stmt).
+         ( p4ctrldecl at level 0, body custom p4stmt).
   Notation "'table' t 'key' ':=' ems 'actions' ':=' acts @ i"
     := (CDTable t {|table_key:=ems; table_actions:=acts|} i)
-         (in custom p4ctrldecl at level 0).
+         ( p4ctrldecl at level 0).
 End ControlNotations.
 
 Module TopDeclNotations.
   Import TopDecl.
   
   Notation "'%{' decl '}%'" := decl (decl custom p4topdecl at level 99).
-  Notation "( x )" := x (in custom p4topdecl, x at level 99).
+  Notation "( x )" := x ( p4topdecl, x at level 99).
   Notation "x"
-    := x (in custom p4topdecl at level 0, x constr at level 0).
+    := x ( p4topdecl at level 0, x constr at level 0).
   Notation "d1 ';%;' d2 @ i"
     := (TPSeq d1 d2 i)
-         (in custom p4topdecl at level 10,
+         ( p4topdecl at level 10,
              d1 custom p4topdecl, d2 custom p4topdecl,
              right associativity).
   Notation "'Instance' x 'of' c < targs > ( args ) @ i"
-    := (TPInstantiate c x targs args i) (in custom p4topdecl at level 0).
+    := (TPInstantiate c x targs args i) ( p4topdecl at level 0).
   Notation "'void' f < tparams > ( params ) { body } @ i"
     := (TPFunction f tparams {|paramargs:=params; rtrns:=None|} body i)
-         (in custom p4topdecl at level 0, body custom p4stmt).
+         ( p4topdecl at level 0, body custom p4stmt).
   Notation "'fn' f < tparams > ( params ) '->' t { body } @ i"
     := (TPFunction f tparams {|paramargs:=params; rtrns:=Some t|} body i)
-         (in custom p4topdecl at level 0,
+         ( p4topdecl at level 0,
              t custom p4type, body custom p4stmt).
   Notation "'extern' e < tparams > ( cparams ) { methods } @ i"
     := (TPExtern e tparams cparams methods i)
-         (in custom p4topdecl at level 0).
+         ( p4topdecl at level 0).
   Notation "'control' c ( cparams ) ( eps ) ( params ) 'apply' { blk } 'where' { body } @ i"
     := (TPControl c cparams eps params body blk i)
-         (in custom p4topdecl at level 0,
+         ( p4topdecl at level 0,
              blk custom p4stmt, body custom p4ctrldecl).
   Notation "'parser' p ( cparams ) ( eps ) ( params ) 'start' ':=' st { states } @ i"
     := (TPParser p cparams eps params st states i)
-         (in custom p4topdecl at level 0, st custom p4prsrstateblock).
+         ( p4topdecl at level 0, st custom p4prsrstateblock).
 End TopDeclNotations.
 
 Module AllCubNotations.
